Some lemmas about term neutral forms and IsType

SystemFD/Term/Substitution.lean
@@ -66,25 +66,6 @@ namespace Term
   | [] => base
   | .cons k ks => k -k> (mk_kind_arrow base ks)
 
-  theorem kind_arrow_lemma : split_kind_arrow κ = .some (κs, ret_κ) ->
-      mk_kind_arrow ret_κ κs = κ := by
-  intros h
-  induction κs generalizing κ ret_κ <;> simp at *
-  induction κ <;> simp at *
-  cases h; rfl
-  case _ v _ _ ih1 ih2 => sorry
-  case _ k ks ih =>
-  unfold Term.split_kind_arrow_aux at h
-  sorry
-
-
-  theorem mk_kind_arrow_lemma :  mk_kind_arrow ret_κ κs = κ ->
-    split_kind_arrow κ = .some (κs, ret_κ) := by
-  intro j
-  induction κs
-  simp; rw[<-j]; simp; sorry
-  sorry
-
 
   @[simp]
   def mk_kind_app : Nat -> List Term -> Term := λ h sp =>
@@ -93,7 +74,7 @@ namespace Term
   @[simp]
   def mk_kind_app_rev (acc : Term) : List Term -> Term
   | [] => acc
-  | .cons a as => mk_kind_app_rev (acc `@ a) as
+  | .cons a as => (mk_kind_app_rev acc as) `@k a
 
   theorem apply_spine_peel_term :
     apply_spine f (sp ++ [(.term, a)]) = (apply_spine f sp `@ a)
