Hs/HsTerm/Shape.lean
@@ -20,6 +20,34 @@ namespace HsTerm
   | all : IsKind A -> IsType B -> IsType (`∀{A} B)
   | arrow : IsType A -> IsType B -> IsType (A → B)
   | farrow : IsType A -> IsType B -> IsType (A ⇒ B)
-  | app : IsType A -> IsType B -> IsType (f `•k a)
+  | app : IsType A -> IsType B -> IsType (A `•k B)
+
+
+theorem hs_type_neutral_form_is_type (τ : HsTerm) :
+  τ.IsType ->
+  τ.neutral_form = .some (h, sp) ->
+  h.IsType ∧ ∀ k ∈ sp, k.2.IsType := by
+  intros h1 h2
+  induction h1 generalizing h sp <;> simp at *
+  case _ => cases h2; case _ h2 h3 =>
+    cases h2; cases h3;
+    constructor;constructor; simp
+  case _ ih1 ih2 =>
+    rw[Option.bind_eq_some] at h2; cases h2
+    case _ h2 =>
+    cases h2; case _ h2 h3 =>
+    cases h3
+    have ih1' := ih1 h2
+    cases ih1'
+    constructor; assumption
+    intros; case _ h =>
+    simp at h;
+    cases h
+    case _ ih a b h =>
+      apply ih a b h
+    case _ h =>
+    cases h; case _ e1 e2 =>
+    cases e1; cases e2
+    assumption
 
 end HsTerm
